## 1 Manual solution to minimum failing example

### 1.1 Notation

- $\Delta t$ : time step, set to 1 to simplify the minimm failing example.
- $\Delta x$ : cell width, set to 1 to simpilfy the minimum failing example.
- $u_{i, j}$ : Evolving variable at cell $i$, time $j$. $u$ is arranged on a 1-D grid with 2 cells.
- $u_{i-, j}$ : Face value of left (west) face of cell $i$
- $u_{i+, j}$ : Face value of right (east) face of cell $i$
- $u_{g}$ : ghost cell on the right end of the mesh
- $\alpha_{i-}$ or $\alpha_{i+}$ : The $\alpha$ weight to use on $u_{i}$ when calculating the face value $u_{i-}$ or $u_{i+}$ for a convection term
- $v$ : Convection strength on faces: $[0,1,1]$


### 1.2 Problem definition

We want to solve

$$
\frac{d u}{d t}=-\nabla \cdot(v u)
$$

subject to a boundary condition that

$$
u_{0-}=1, u_{1+}=1
$$

using the implicit method, for one time step, stepping from $t=0$ to $t=1$ for simplicity.

The implicit method discretization using $\Delta t=1$ is:

$$
\begin{aligned}
& u_{0,1}-F_{0,1}=u_{0,0} \\
& u_{1,1}-F_{1,1}=u_{1,0}
\end{aligned}
$$

where $F$ is the contribution of the convection term to the linear system.

$$
\rightarrow \quad \begin{aligned}
& u_{0,1}=F_{0,1}+u_{0,0} \\
& u_{1,1}=F_{1,1}+u_{1,0}
\end{aligned}
$$

Expanding $F$ to define the contribution of the convection term, using $\Delta x=1$ to keep the expression simple, we get:

$$
\begin{aligned}
& u_{0,1}=v_{0} u_{0-, 1}-v_{1} u_{0+, 1}+u_{0,0} \\
& u_{1,1}=v_{1} u_{1-, 1}-v_{2} u_{1+, 1}+u_{1,0}
\end{aligned}
$$

Filling in concrete values for $v$ we obtain:

$$
\begin{gathered}
u_{0,1}=-u_{0+, 1}+u_{0,0} \\
u_{1,1}=u_{1-, 1}-u_{1+, 1}+u_{1,0}
\end{gathered}
$$

Filling in $u_{1+, 1} \equiv 1$ from the boundary condition:

$$
\begin{gathered}
u_{0,1}=-u_{0+, 1}+u_{0,0} \\
u_{1,1}=u_{1-, 1}-1+u_{1,0}
\end{gathered}
$$

Using $\alpha$ weighting to calculate internal face values:

$$
\begin{gathered}
u_{0,1}=-\alpha_{0+} u_{0,1}+\left(1-\alpha_{0+}\right) u_{1,1}+u_{0,0} \\
u_{1,1}=\alpha_{1-} u_{1,1}+\left(1-\alpha_{1-}\right) u_{0,1}-1+u_{1,0}
\end{gathered}
$$

Substituting in $\alpha_{0+}=1$ and $\alpha_{1-}=0$ we get:

$$
\begin{gathered}
u_{0,1}=-u_{0,1}+u_{0,0} \\
u_{1,1}=u_{0,1}-1+u_{1,0}
\end{gathered}
$$

Solving this, we get

$$
\begin{gathered}
u_{0,1}=\frac{u_{0,0}}{2} \\
u_{1,1}=u_{0,1}-1+u_{1,0}
\end{gathered}
$$

Starting from initial conditions of $u=[0,0]$ this gives $[0,-1]$ but FiPy returns $[0,0]$.
(I do obtain $[0,0]$ however if I calculated $u_{1+, 1}$ above using $\alpha$ weighting on a ghost cell, though that's probably not the only valid way to obtain $[0,0]$ )

